mark-and-sweep/spec/GC.Spec.ChunkedMarkBounded.StackStep.fst
@@ -1,0 +1,262 @@
+module GC.Spec.ChunkedMarkBounded.StackStep
+
+module U64 = FStar.UInt64
+module Seq = FStar.Seq
+
+open GC.Spec.Base
+
+module Header = GC.Lib.Header
+module MH = GC.Spec.MajorHeap
+module SweepDefs = GC.Spec.ChunkedSweepCoalesce.Defs
+module MarkDefs = GC.Spec.ChunkedMark.Defs
+module MarkPres = GC.Spec.ChunkedMark.Preservation
+module SpecMark = GC.Spec.Mark
+module BDefs = GC.Spec.ChunkedMarkBounded.Defs
+module BPres = GC.Spec.ChunkedMarkBounded.Preservation
+module BReady = GC.Spec.ChunkedMarkBounded.TargetReady
+module SeqMem = GC.Spec.SeqMemLemmas
+
+#set-options "--z3rlimit 5 --fuel 1 --ifuel 1 --split_queries always --warn_error -321"
+
+let seq_tail_mem (#a:eqtype) (s: Seq.seq a) (x: a)
+  : Lemma
+      (requires Seq.length s > 0 /\ Seq.mem x (Seq.tail s))
+      (ensures Seq.mem x s)
+  =
+  let hd = Seq.head s in
+  let tl = Seq.tail s in
+  assert (s == Seq.cons hd tl);
+  FStar.Seq.Properties.lemma_mem_append (Seq.create 1 hd) tl
+
+let chunked_is_white_not_gray
+    (mh: MH.major_heap)
+    (obj: obj_addr)
+  : Lemma
+      (requires SweepDefs.chunked_is_white mh obj)
+      (ensures ~(BDefs.chunked_is_gray mh obj))
+  =
+  BDefs.chunked_is_gray_step mh obj;
+  if BDefs.chunked_is_gray mh obj then begin
+    SweepDefs.chunked_is_white_read_header mh obj;
+    SweepDefs.chunked_color_of_object_elim mh obj Header.Gray;
+    match SweepDefs.chunked_read_header mh obj with
+    | None -> assert False
+    | Some hdr ->
+      assert (SweepDefs.chunked_color_of_object mh obj == Some Header.Gray);
+      assert (GC.Spec.Object.getColor hdr == Header.Gray);
+      assert (GC.Spec.Object.getColor hdr == Header.White);
+      assert False
+  end
+
+let stack_gray_to_color
+    (mh: MH.major_heap)
+    (st: Seq.seq obj_addr)
+    (target: obj_addr)
+  : Lemma
+      (requires
+        BReady.chunked_stack_points_to_gray mh st /\
+        Seq.mem target st)
+      (ensures
+        SweepDefs.chunked_color_of_object mh target == Some Header.Gray)
+  =
+  BReady.chunked_stack_points_to_gray_elim mh st target;
+  BDefs.chunked_is_gray_step mh target
+
+let make_gray_preserves_stack_gray
+    (mh: MH.major_heap)
+    (child: obj_addr)
+    (st: Seq.seq obj_addr)
+  : Lemma
+      (requires
+        MH.well_formed_major_heap mh /\
+        Seq.mem child (MH.major_objects mh) /\
+        BReady.chunked_stack_points_to_gray mh st)
+      (ensures
+        BReady.chunked_stack_points_to_gray
+          (MarkDefs.chunked_make_gray mh child) st)
+  =
+  let each (target: obj_addr)
+    : Lemma
+        (requires Seq.mem target st)
+        (ensures BDefs.chunked_is_gray (MarkDefs.chunked_make_gray mh child) target)
+    =
+    if target = child then begin
+      MarkPres.chunked_make_gray_makes_gray mh child;
+      BDefs.chunked_is_gray_step (MarkDefs.chunked_make_gray mh child) target
+    end else begin
+      stack_gray_to_color mh st target;
+      MarkPres.chunked_make_gray_preserves_other_gray mh child target;
+      BDefs.chunked_is_gray_step (MarkDefs.chunked_make_gray mh child) target
+    end
+  in
+  FStar.Classical.forall_intro (FStar.Classical.move_requires each);
+  BReady.chunked_stack_points_to_gray_intro (MarkDefs.chunked_make_gray mh child) st
+
+let make_black_preserves_tail_stack_gray
+    (mh: MH.major_heap)
+    (st: Seq.seq obj_addr)
+  : Lemma
+      (requires
+        Seq.length st > 0 /\
+        SpecMark.stack_no_dups st /\
+        BReady.chunked_stack_points_to_gray mh st)
+      (ensures
+        BReady.chunked_stack_points_to_gray
+          (MarkDefs.chunked_make_black mh (Seq.head st)) (Seq.tail st))
+  =
+  let head = Seq.head st in
+  let tail = Seq.tail st in
+  let each (target: obj_addr)
+    : Lemma
+        (requires Seq.mem target tail)
+        (ensures BDefs.chunked_is_gray (MarkDefs.chunked_make_black mh head) target)
+    =
+    assert (~(Seq.mem head tail));
+    assert (target <> head);
+    seq_tail_mem st target;
+    stack_gray_to_color mh st target;
+    MarkPres.chunked_make_black_preserves_other_gray mh head target;
+    BDefs.chunked_is_gray_step (MarkDefs.chunked_make_black mh head) target
+  in
+  FStar.Classical.forall_intro (FStar.Classical.move_requires each);
+  BReady.chunked_stack_points_to_gray_intro
+    (MarkDefs.chunked_make_black mh head) tail
+
+let stack_no_dups_tail
+    (st: Seq.seq obj_addr)
+  : Lemma
+      (requires
+        Seq.length st > 0 /\
+        SpecMark.stack_no_dups st)
+      (ensures SpecMark.stack_no_dups (Seq.tail st))
+  = ()
+
+let rec chunked_push_children_bounded_preserves_bounded_stack_props
+    (mh: MH.major_heap)
+    (st: Seq.seq obj_addr)
+    (obj: obj_addr)
+    (i: U64.t{U64.v i >= 1})
+    (ws: U64.t)
+    (cap: nat)
+  : Lemma
+      (requires
+        MH.well_formed_major_heap mh /\
+        BPres.chunked_push_children_bounded_preservation_ready mh obj i ws /\
+        BReady.chunked_bounded_stack_props mh st)
+      (ensures
+        (let (mh', st') =
+          BDefs.chunked_push_children_bounded mh st obj i ws cap in
+         BReady.chunked_bounded_stack_props mh' st'))
+      (decreases (U64.v ws - U64.v i))
+  =
+  BReady.chunked_bounded_stack_props_objects mh st;
+  BReady.chunked_bounded_stack_props_gray mh st;
+  BReady.chunked_bounded_stack_props_no_dups mh st;
+  if U64.v i > U64.v ws then
+    BDefs.chunked_push_children_bounded_done mh st obj i ws cap
+  else begin
+    assert (U64.v i <= U64.v ws);
+    BDefs.chunked_push_children_bounded_step mh st obj i ws cap;
+    let v = MarkDefs.chunked_get_field mh obj i in
+    if MarkDefs.chunked_is_pointer_field mh v then begin
+      let child_raw = MarkDefs.chunked_pointer_field_as_obj_addr mh v in
+      let child = MarkDefs.chunked_resolve_object mh child_raw in
+      if SweepDefs.chunked_is_white mh child then begin
+        let mh_gray = MarkDefs.chunked_make_gray mh child in
+        BPres.chunked_push_children_bounded_preservation_ready_child
+          mh obj i ws;
+        MarkPres.chunked_make_gray_preserves_major_objects mh child;
+        MarkPres.chunked_make_gray_preserves_well_formed mh child;
+        MarkPres.stack_objects_in_major_preserved_by_major_objects
+          mh mh_gray st;
+        make_gray_preserves_stack_gray mh child st;
+        BReady.chunked_bounded_stack_props_intro mh_gray st;
+        if Seq.mem child st then begin
+          BReady.chunked_stack_points_to_gray_elim mh st child;
+          chunked_is_white_not_gray mh child;
+          assert False
+        end;
+        let st' =
+          if Seq.length st < cap then begin
+            BReady.chunked_stack_objects_in_major_cons mh_gray child st;
+            MarkPres.chunked_make_gray_makes_gray mh child;
+            BDefs.chunked_is_gray_step mh_gray child;
+            BReady.chunked_stack_points_to_gray_cons mh_gray child st;
+            assert (Seq.head (Seq.cons child st) == child);
+            assert (Seq.equal (Seq.tail (Seq.cons child st)) st);
+            Seq.lemma_eq_elim (Seq.tail (Seq.cons child st)) st;
+            assert (Seq.tail (Seq.cons child st) == st);
+            assert (~ (Seq.mem
+              (Seq.head (Seq.cons child st))
+              (Seq.tail (Seq.cons child st))));
+            assert (SpecMark.stack_no_dups (Seq.tail (Seq.cons child st)));
+            assert (SpecMark.stack_no_dups (Seq.cons child st));
+            BReady.chunked_bounded_stack_props_intro mh_gray (Seq.cons child st);
+            Seq.cons child st
+          end else
+            st in
+        if U64.v i < U64.v ws then
+          BPres.chunked_push_children_bounded_preservation_ready_next
+            mh obj i ws;
+        if U64.v i < U64.v ws then
+          chunked_push_children_bounded_preserves_bounded_stack_props
+            mh_gray st' obj (U64.add i 1UL) ws cap
+      end else if U64.v i < U64.v ws then begin
+        BPres.chunked_push_children_bounded_preservation_ready_next
+          mh obj i ws;
+        chunked_push_children_bounded_preserves_bounded_stack_props
+          mh st obj (U64.add i 1UL) ws cap
+      end
+    end else if U64.v i < U64.v ws then begin
+      BPres.chunked_push_children_bounded_preservation_ready_next
+        mh obj i ws;
+      chunked_push_children_bounded_preserves_bounded_stack_props
+        mh st obj (U64.add i 1UL) ws cap
+    end
+  end
+
+let chunked_mark_step_bounded_preserves_bounded_stack_props
+    (mh: MH.major_heap)
+    (st: Seq.seq obj_addr)
+    (cap: nat)
+  : Lemma
+      (requires
+        Seq.length st > 0 /\
+        MH.well_formed_major_heap mh /\
+        BPres.chunked_mark_step_bounded_preservation_ready mh st cap /\
+        BReady.chunked_bounded_stack_props mh st)
+      (ensures
+        (let (mh', st') =
+          BDefs.chunked_mark_step_bounded mh st cap in
+         BReady.chunked_bounded_stack_props mh' st'))
+  =
+  let obj = Seq.head st in
+  let tail = Seq.tail st in
+  BReady.chunked_bounded_stack_props_objects mh st;
+  BReady.chunked_bounded_stack_props_gray mh st;
+  BReady.chunked_bounded_stack_props_no_dups mh st;
+  BReady.chunked_bounded_stack_head mh st;
+  MarkPres.stack_objects_in_major_tail mh st;
+  stack_no_dups_tail st;
+  if MarkDefs.chunked_is_no_scan mh obj then begin
+    BDefs.chunked_mark_step_bounded_no_scan mh st cap;
+    MarkPres.chunked_make_black_preserves_major_objects mh obj;
+    MarkPres.stack_objects_in_major_preserved_by_major_objects
+      mh (MarkDefs.chunked_make_black mh obj) tail;
+    make_black_preserves_tail_stack_gray mh st;
+    BReady.chunked_bounded_stack_props_intro
+      (MarkDefs.chunked_make_black mh obj) tail
+  end else begin
+    let mh_black = MarkDefs.chunked_make_black mh obj in
+    let ws = SweepDefs.chunked_wosize_of_object mh obj in
+    BPres.chunked_mark_step_bounded_preservation_ready_scan mh st cap;
+    BDefs.chunked_mark_step_bounded_scan mh st cap;
+    MarkPres.chunked_make_black_preserves_major_objects mh obj;
+    MarkPres.chunked_make_black_preserves_well_formed mh obj;
+    MarkPres.stack_objects_in_major_preserved_by_major_objects
+      mh mh_black tail;
+    make_black_preserves_tail_stack_gray mh st;
+    BReady.chunked_bounded_stack_props_intro mh_black tail;
+    chunked_push_children_bounded_preserves_bounded_stack_props
+      mh_black tail obj 1UL ws cap
+  end
